added cst + synth for lvalues

C0deine/Type/Typ.lean
@@ -11,8 +11,6 @@ mutual
 inductive Typ
 | prim (p : Typ.Primitive)
 | mem (m : Typ.Memory)
-| void_star
-| any
 deriving Inhabited, Hashable
 
 inductive Typ.Memory
@@ -21,6 +19,11 @@ inductive Typ.Memory
 | struct (sym : Symbol)
 deriving Inhabited, Hashable
 end
+
+inductive Typ.Check
+| type : Typ → Typ.Check
+| void
+| any
 
 namespace Typ
 
@@ -31,67 +34,72 @@ instance : ToString Primitive where toString := Primitive.toString
 
 mutual
 def Memory.toString : Typ.Memory → String
-  | .pointer (typ : Typ)   => s!"{Typ.toString typ} *"
-  | .array (typ : Typ)     => s!"{Typ.toString typ}[]"
+  | .pointer (typ : Typ)   => s!"{toString typ} *"
+  | .array (typ : Typ)     => s!"{toString typ}[]"
   | .struct (sym : Symbol) => s!"struct {sym}"
 
 def toString : Typ → String
-  | prim (p : Primitive) => Primitive.toString p
+  | .prim (p : Primitive) => Primitive.toString p
   | .mem (m : Typ.Memory) => Memory.toString m
-  | .void_star => "void *"
-  | .any => "'any"
 end
 
-instance : ToString Typ.Memory where toString := Typ.Memory.toString
+def Check.toString : Check → String
+  | .type t => s!"{Typ.toString t}"
+  | .void => "'void"
+  | .any => "'any"
+
+instance : ToString Memory where toString := Memory.toString
 instance : ToString Typ where toString := Typ.toString
+instance : ToString Typ.Check where toString := Typ.Check.toString
 
 mutual
 -- encoding structural equality
-def deq (a b : Typ) : Decidable (a = b) :=
+def structEq (a b : Typ) : Bool :=
   match a, b with
-  | .prim p1, .prim p2 =>
-    match decEq p1 p2 with
-    | isTrue h  => isTrue  <| h ▸ rfl
-    | isFalse h => isFalse <| fun h' => by simp at h'; apply h h'
-  | .mem m1, .mem m2 =>
-    match Typ.Memory.deq m1 m2 with
-    | isTrue h  => isTrue  <| h ▸ rfl
-    | isFalse h => isFalse <| fun h' => by simp at h'; apply h h'
-  | .void_star, .void_star =>
-    isTrue <| Eq.refl Typ.void_star
-  | .any, .any =>
-    isTrue <| Eq.refl Typ.any
-  | _, _ => sorry
-    -- isFalse <| fun h => _
+  | .prim p1, .prim p2 => p1 = p2
+  | .mem m1, .mem m2 => Memory.structEq m1 m2
+  | _, _ => false
 
-def Memory.deq (a b : Typ.Memory) : Decidable (a = b) :=
+def Memory.structEq (a b : Memory) : Bool :=
   match a, b with
-  | .struct s1, .struct s2 =>
-    match decEq s1 s2 with
-    | isTrue h  => isTrue  <| h ▸ rfl
-    | isFalse h => isFalse <| fun h' => by simp at h'; apply h h'
-  | .pointer t1, .pointer t2 =>
-    match Typ.deq t1 t2 with
-    | isTrue h  => isTrue  <| h ▸ rfl
-    | isFalse h => isFalse <| fun h' => by simp at h'; apply h h'
-  | .array t1, .array t2 =>
-    match Typ.deq t1 t2 with
-    | isTrue h  => isTrue  <| h ▸ rfl
-    | isFalse h => isFalse <| fun h' => by simp at h'; apply h h'
-  | _, _ => sorry
-    -- isFalse <| _
+  | .struct s1, .struct s2 => s1 = s2
+  | .pointer t1, .pointer t2 => Typ.structEq t1 t2
+  | .array t1, .array t2 => Typ.structEq t1 t2
+  | _, _ => false
 end
 
-instance : DecidableEq Typ.Memory := Typ.Memory.deq
-instance : DecidableEq Typ := Typ.deq
+mutual
+theorem deq {a b : Typ} : structEq a b = true ↔ a = b := by
+  cases a <;> cases b <;>
+  ( unfold structEq
+    simp
+    try apply Memory.deq
+  )
+
+theorem Memory.deq {a b : Memory} : Memory.structEq a b = true ↔ a = b := by
+  cases a <;> cases b <;>
+  ( unfold Memory.structEq
+    simp
+    try apply Typ.deq
+  )
+end
+
+instance : DecidableEq Typ := fun a b =>
+  match Bool.decEq (Typ.structEq a b) true with
+  | .isTrue h  => .isTrue (Typ.deq.mp h)
+  | .isFalse h => .isFalse (h ∘ Typ.deq.mpr)
+instance : DecidableEq Memory := fun a b =>
+  match Bool.decEq (Memory.structEq a b) true with
+  | .isTrue h  => .isTrue (Memory.deq.mp h)
+  | .isFalse h => .isFalse (h ∘ Memory.deq.mpr)
+
+deriving instance DecidableEq for Typ.Check
 
 mutual
   def equiv (a b : Typ) : Bool :=
     match a, b with
     | .prim p1  , .prim p2    => p1 == p2
     | .mem m1   , .mem m2     => Memory.equiv m1 m2
-    | .void_star, .void_star  => true
-    | .any, _ | _, .any       => true
     | _, _                    => false
 
   def Memory.equiv (a b : Memory) : Bool :=
@@ -102,33 +110,26 @@ mutual
     | _, _                     => false
 end
 
-instance : BEq Typ where beq := equiv
-instance : BEq Memory where beq := Memory.equiv
-
--- A type is reduced if it contains no "any"
--- todo: do we need to lookup the symbol for structures?
-mutual
-inductive Reduced : Typ → Prop where
-| prim_int_reduced : Reduced (Typ.prim Typ.Primitive.int)
-| prim_bool_reduced : Reduced (Typ.prim Typ.Primitive.bool)
-| mem_reduced : ∀ m, Memory.Reduced m → Reduced (Typ.mem m)
-| void_reduced : Reduced Typ.void_star
-
-inductive Memory.Reduced : Memory → Prop where
-| pointer_reduced : ∀ t, Reduced t → Memory.Reduced (Typ.Memory.pointer t)
-| array_reduced   : ∀ t, Reduced t → Memory.Reduced (Typ.Memory.array t)
-| struct_reduced  : ∀ s, Memory.Reduced (Typ.Memory.struct s)
-end
-
-theorem Reduced.not_any : ¬ Reduced (Typ.any) := fun h => nomatch h
+def Check.equiv (a b : Check) : Bool :=
+  match a, b with
+  | .type t1, .type t2  => Typ.equiv t1 t2
+  | .void, .void        => true
+  | .any, _ | _, .any   => true
+  | _, _ => false
 
 def isScalar : Typ → Bool
   | .prim .int => true
   | .prim .bool => true
   | _ => false
+def Check.isScalar : Typ.Check → Bool
+  | .type t => t.isScalar
+  | _ => false
 
 def isSmall : Typ → Bool
   | .mem (.struct _) => false
+  | _ => true
+def Check.isSmall : Typ.Check → Bool
+  | .type t => t.isSmall
   | _ => true
 
 def sizeof : Typ → Option Nat
@@ -137,7 +138,7 @@ def sizeof : Typ → Option Nat
   | .mem (.pointer _) => some 8
   | .mem (.array _) => some 8
   | .mem (.struct _) => none
-  | .void_star => some 8
+def Check.sizeof : Typ.Check → Option Nat
+  | .type t => t.sizeof
   | _ => none
-
 end Typ
